Test/dafny0/Trait/TraitOverride2.dfy
@@ -10,29 +10,34 @@ trait Spec<U> {
     requires done || hasFailed || (!done && !hasFailed)  // tantamount to "true"
     reads this, Repr
     ensures Valid() ==> this in Repr
-    decreases this, Repr
+    decreases Repr
 
   method DoIt() returns (u: U)
     requires Valid()
     modifies Repr
     ensures Valid()
     ensures Repr == old(Repr)
-    decreases this, Repr
+    decreases Repr
 }
 
 class Impl<T> extends Spec<T> {
   const tt: T
   var n: nat
 
-  constructor (t: T) {
+  constructor (t: T)
+    ensures Valid()
+  {
     tt, n := t, 0;
+    Repr := {this};
+    new;
+    assert this in Repr;
   }
 
   predicate Valid()
     requires done || hasFailed || (!done && !hasFailed)
     reads this, Repr
     ensures Valid() ==> this in Repr
-    decreases this, Repr
+    decreases Repr
   {
     this in Repr
   }
@@ -42,7 +47,7 @@ class Impl<T> extends Spec<T> {
     modifies Repr
     ensures Valid()
     ensures Repr == old(Repr)
-    decreases this, Repr
+    decreases Repr
   {
     if done || hasFailed {
       // nothing else to do
@@ -58,11 +63,41 @@ class Impl<T> extends Spec<T> {
   }
 }
 
-class FixedImpl extends Spec<int> {
+class AnotherImpl<T> extends Spec<seq<T>> {
+  constructor ()
+    ensures Valid()
+  {
+    Repr := {this};
+    new;
+    assert this in Repr;  // this had once failed
+  }
+
   predicate Valid()
     reads this, Repr
     ensures Valid() ==> this in Repr
-    decreases this, Repr
+    decreases Repr
+  { this in Repr }
+
+  method DoIt() returns (u: seq<T>)
+    requires Valid()
+    modifies Repr
+    ensures Valid()
+    ensures Repr == old(Repr)
+    decreases Repr
+  { }
+}
+
+class FixedImpl extends Spec<int> {
+  constructor (arr: array<real>)
+    ensures Valid()
+  {
+    Repr := {this, arr};
+  }
+
+  predicate Valid()
+    reads this, Repr
+    ensures Valid() ==> this in Repr
+    decreases Repr
   {
     this in Repr
   }
@@ -72,5 +107,5 @@ class FixedImpl extends Spec<int> {
     modifies Repr
     ensures Valid()
     ensures Repr == old(Repr)
-    decreases this, Repr
+    decreases Repr
 }
